Implementing progress.

src/All.v
@@ -1,11 +1,12 @@
-Require HJ.AsyncFinish.Lang.
-Module F := HJ.AsyncFinish.Lang.
+Require HJ.AsyncFinish.Syntax.
+Module F := HJ.AsyncFinish.Syntax.
 Require HJ.Phasers.Lang.
 Module P := HJ.Phasers.Lang.
 Require Import HJ.Vars.
 Require Import HJ.AsyncFinish.IEF.
 
 Notation fstate := (Map_FID.t P.phasermap).
+
 
 Inductive state := mk_state {
   get_finish: F.finish;
@@ -24,8 +25,8 @@ Definition set_finish (s:state) (f:F.finish) : state :=
 Module Semantics.
 
 Require Import HJ.Phasers.Lang.
-Import F.Semantics.
-Module FS := F.Semantics.
+Require HJ.AsyncFinish.Semantics.
+Module FS := HJ.AsyncFinish.Semantics.
 
 Inductive op := 
   | BEGIN_ASYNC : list phased -> tid -> op
@@ -45,15 +46,58 @@ Inductive packet :=
 
 Definition translate (o:op) : packet :=
   match o with
+  (* Copies registry from spawner and registers task in finish scope of spawner*)
   | BEGIN_ASYNC ps t => both (P.ASYNC ps t) (FS.BEGIN_ASYNC t)
-  | END_ASYNC => both (P.DROP_ALL) (FS.END_ASYNC)
+  (* Drops all phasers and removes task from finish scope *)
+  | END_ASYNC => both P.DROP_ALL FS.END_ASYNC
+  (* Pushes a finish scope  *)
   | BEGIN_FINISH => only_f FS.BEGIN_FINISH
-  | END_FINISH => only_f FS.END_FINISH
+  (* Drops all phasers and pops a finish scope *)
+  | END_FINISH => both P.DROP_ALL FS.END_FINISH
+  (* Phaser-only operations: *)
   | PH_NEW p => only_p (P.PH_NEW p)
   | PH_SIGNAL p => only_p (P.PH_SIGNAL p)
   | PH_DROP p => only_p (P.PH_DROP p)
-  | SIGNAL_ALL => only_p (P.SIGNAL_ALL)
-  | WAIT_ALL => only_p (P.WAIT_ALL)
+  | SIGNAL_ALL => only_p P.SIGNAL_ALL
+  | WAIT_ALL => only_p P.WAIT_ALL
+  end.
+
+Definition as_f_op (o:op) :=
+  match translate o with
+  | only_f o => Some o
+  | both _ o => Some o
+  | only_p _ => None
+  end.
+
+Lemma translate_only_f_impl_as_f_op:
+  forall i o,
+  translate i = only_f o ->
+  as_f_op i = Some o.
+Proof.
+  intros; destruct i; try (simpl in *; inversion H); compute; auto.
+Qed.
+
+Lemma translate_both_impl_as_f_op:
+  forall i o o',
+  translate i = both o o' ->
+  as_f_op i = Some o'.
+Proof.
+  intros; destruct i; try (simpl in *; inversion H); compute; auto.
+Qed.
+
+Lemma translate_only_p_impl_as_f_op:
+  forall i o,
+  translate i = only_p o ->
+  as_f_op i = None.
+Proof.
+  intros; destruct i; try (simpl in *; inversion H); compute; auto.
+Qed.
+
+Definition as_p_op (o:op) :=
+  match translate o with
+  | only_p o => Some o
+  | both o _ => Some o
+  | only_f _ => None
   end.
 
 Inductive PhasermapOf (s:state) (t:tid) (f:fid) (m:phasermap) : Prop :=
@@ -61,25 +105,218 @@ Inductive PhasermapOf (s:state) (t:tid) (f:fid) (m:phasermap) : Prop :=
     FID (get_finish s) t f ->
     Map_FID.MapsTo f m s.(get_fstate) ->
     PhasermapOf s t f m.
+(*
+Structure context := mk_context {
+  get_phasermap: P.phasermap;
+  get_finish: F.finish;
+}.
+*)
+Definition context := (P.phasermap * F.finish) % type.
+Inductive ContextOf (s:state) (t:tid) : context -> Prop :=
+  context_of_def:
+    forall f m,
+    PhasermapOf s t f m ->
+    ContextOf s t (m, (get_finish s)).
+
+Inductive CtxReduce (ctx:context) (t:tid) (o:op) : context -> Prop :=
+  | reduce_p:
+    forall m o',
+    translate o = only_p o' ->
+    P.Reduce (fst ctx) t o' m ->
+    CtxReduce ctx t o (m, snd ctx)
+  | reduce_f:
+    forall f o',
+    translate o = only_f o' ->
+    FS.Reduce (snd ctx) t o' f ->
+    CtxReduce ctx t o (fst ctx, f)
+  | reduce_both:
+    forall m o' f o'',
+    translate o = both o' o'' ->
+    P.Reduce (fst ctx) t o' m ->
+    FS.Reduce (snd ctx) t o'' f ->
+    CtxReduce ctx t o (m, f).
 
 Inductive Reduce (s:state) (t:tid) (o:op) : state -> Prop :=
-  | reduce_p:
-    forall f m m' o',
+  reduce_def:
+    forall f m ctx,
     PhasermapOf s t f m ->
-    translate o = only_p o' ->
-    P.Reduce m t o' m' ->
-    Reduce s t o (put_phasermap s f m')
-  | reduce_f:
-    forall f' o',
-    translate o = only_f o' ->
-    FS.Reduce (get_finish s) t o' f' ->
-    Reduce s t o (set_finish s f')
-  | reduce_both:
-    forall m i m' o' f' o'',
-    translate o = both o' o'' ->
-    PhasermapOf s t i m ->
-    P.Reduce m t o' m' ->
-    FS.Reduce (get_finish s) t o'' f' ->
-    Reduce s t o
-      (set_finish (put_phasermap s i m') f').
+    CtxReduce (m, get_finish s) t o ctx ->
+    Reduce s t o (set_finish (put_phasermap s f (fst ctx)) (snd ctx)).
+
 End Semantics.
+
+
+Module Typesystem.
+  Import Semantics.
+  Require HJ.Phasers.Typesystem.
+  Require HJ.AsyncFinish.Typesystem.
+  Module P_T := HJ.Phasers.Typesystem.
+  Module F_T := HJ.AsyncFinish.Typesystem.
+  
+  Inductive Check (ctx:context) (t:tid): op -> Prop :=
+  | check_only_p:
+    forall i o,
+    translate i = only_p o ->
+    P_T.Check (fst ctx) t o ->
+    Check ctx t i
+  | check_only_f:
+    forall i o,
+    translate i = only_f o ->
+    F_T.Check (snd ctx) t o ->
+    Check ctx t i
+  | check_both:
+    forall i o o',
+    translate i = both o o' ->
+    F_T.Check (snd ctx) t o' ->
+    P_T.Check (fst ctx) t o ->
+    Check ctx t i.
+
+  Lemma check_inv_f_check:
+    forall p f t i o,
+    Check (p, f) t i ->
+    as_f_op i = Some o ->
+    F_T.Check f t o.
+  Proof.
+    intros.
+    inversion H; (subst; simpl in *).
+    - apply translate_only_p_impl_as_f_op in H1.
+      rewrite H1 in H0.
+      inversion H0.
+    - apply translate_only_f_impl_as_f_op in H1.
+      rewrite H1 in H0.
+      inversion H0.
+      subst.
+      assumption.
+    - apply translate_both_impl_as_f_op in H1.
+      rewrite H1 in H0.
+      inversion H0.
+      subst.
+      assumption.
+  Qed.
+
+End Typesystem.
+
+Require HJ.Phasers.Progress.
+Module P_P := HJ.Phasers.Progress.
+
+Module Progress.
+  Import Semantics.
+  Import Typesystem.
+  Definition requests := Map_TID.t op.
+  Definition r_state := (state * requests) % type.
+
+  Inductive Redex (s:r_state) (t:tid) (i:op) (s':state) : Prop :=
+    redex_def:
+      Map_TID.MapsTo t i (snd s) ->
+      Reduce (fst s) t i s' ->
+      Redex s t i s'.
+
+  Section SimpleProgress.
+    Variable f:F.finish.
+    Variable f_IsValid: F_T.Valid f.
+    Variable p:P.phasermap.
+    Variable p_IsValid: P_T.Valid p.
+    Variable reqs: Map_TID.t op.
+    Variable ReqsChecked:
+      forall t i,
+      Map_TID.MapsTo t i reqs -> Check (p,f) t i.
+    Require Import HJ.AsyncFinish.Progress.
+    Variable IsFlat:
+      Flat f.
+    Variable p_reqs: Map_TID.t P.op.
+    Variable p_reqs_spec_1:
+      forall t o,
+      Map_TID.MapsTo t o p_reqs ->
+      exists i, Map_TID.MapsTo t i reqs /\ as_p_op i = Some o.
+    Variable p_reqs_spec_2:
+      forall t i o,
+      Map_TID.MapsTo t i reqs ->
+      as_p_op i = Some o ->
+      Map_TID.MapsTo t o p_reqs.
+      
+    Variable f_reqs: Map_TID.t FS.op.
+    Variable f_reqs_spec_1:
+      forall t o,
+      Map_TID.MapsTo t o f_reqs ->
+      exists i, Map_TID.MapsTo t i reqs /\ as_f_op i = Some o.
+    Variable f_reqs_spec_2:
+      forall t i o,
+      Map_TID.MapsTo t i reqs ->
+      as_f_op i = Some o ->
+      Map_TID.MapsTo t o f_reqs.
+    
+    Theorem progress_only_f:
+      forall t i o,
+      Map_TID.MapsTo t i reqs ->
+      translate i = only_f o ->
+      exists f', CtxReduce (p, f) t i (p, f').
+    Proof.
+      intros.
+      assert (Hx := H0).
+      apply translate_only_f_impl_as_f_op in Hx.
+      assert (Hy := Hx).
+      apply f_reqs_spec_2 with (t:=t) in Hx; auto.
+      assert (R: exists f', FS.Reduce f t o f'). {
+        assert (F_T.Check f t o). {
+          eauto using check_inv_f_check.
+        }
+        auto using flat_reduces.
+      }
+      destruct R as (f', R).
+      exists f'.
+      apply reduce_f with (o); auto.
+    Qed.
+    
+    Lemma is_p_impl_reqs_f_spec_1:
+      (forall t i, Map_TID.MapsTo t i reqs ->  exists o, as_p_op i = Some o) ->
+      forall t i,
+      Map_TID.MapsTo t i reqs ->
+      (exists o, as_p_op i = Some o /\ Map_TID.MapsTo t o p_reqs).
+    Proof.
+      intros IsP.
+      intros.
+      assert (Hx := H).
+      apply IsP in H.
+      destruct H as (o, ?).
+      exists o; intuition.
+      eauto.
+    Qed.
+
+
+    Theorem progress_all_p:
+      (forall t i, Map_TID.MapsTo t i reqs ->  exists o, as_p_op i = Some o) ->
+      exists t i ctx, CtxReduce (p, f) t i ctx.
+    Proof.
+      Print progress.
+      
+    Qed.
+    
+
+    Theorem progress:
+      ~ Map_TID.Empty reqs ->
+      exists t i ctx, CtxReduce (p, f) t i ctx.
+    Proof.
+      intros.
+      
+    Qed.
+      
+    Theorem progress:
+      ~ Map_TID.Empty reqs ->
+      exists t i ctx, CtxReduce (p, f) t i ctx.
+    Proof.
+      
+    Qed.
+      
+  Section Progress.
+
+  Variable s: state.
+  Variable reqs: Map_TID.t op.
+  Variable ReqsChecked:
+    forall t i ctx,
+    Map_TID.MapsTo t i reqs -> ContextOf s t ctx -> Check ctx t i.
+
+  Theorem progress:
+    ~ Map_TID.Empty reqs ->
+    exists t i s',
+    Redex (s,reqs) t i s'.
+  Proof.
